Prove cheats

compiler/encoders/ag32/ag32_targetScript.sml
@@ -16,7 +16,7 @@ val ag32_init_regs_def = Define `
 
 val is_ag32_init_state_def = Define `
  is_ag32_init_state mem mem_start s <=>
-  s.PC = mem_start + n2w print_string_max_length /\
+  s.PC = mem_start + n2w (print_string_max_length+1) /\
   s.MEM = mem /\
   s.R = ag32_init_regs mem_start o w2n /\
   s.io_events = []`;
